\documentclass[fleqn]{article}
\oddsidemargin 0.0in
\textwidth 6.0in
\thispagestyle{empty}
\usepackage{import}
\usepackage{amsmath}
\usepackage{graphicx}
\usepackage[english]{babel}
\usepackage[utf8x]{inputenc}
\usepackage{float}
\usepackage{bigints}
\usepackage[colorinlistoftodos]{todonotes}

\definecolor{hwColor}{HTML}{AD53BA}

\begin{document}

  \begin{titlepage}

    \newcommand{\HRule}{\rule{\linewidth}{0.5mm}} % Defines a new command for the horizontal lines, change thickness here

    \center % Center everything on the page
    


    \textsc{\LARGE Arizona State University}\\[1.5cm] % Name of your university/college

    \textsc{\LARGE Mathematical Methods For Physics I }\\[1.5cm] % Major heading such as course name


    \begin{figure}
      \includegraphics[width=\linewidth]{asu.png}
    \end{figure}


    \HRule \\[0.4cm]
    { \huge \bfseries Homework 9}\\[0.4cm] 
    \HRule \\[1.5cm]
    
    \textbf{Behnam Amiri}

    \bigbreak

    \textbf{Prof: Cecilia Lunardini}

    \bigbreak


    \textbf{{\large \today}\\[2cm]}

    \vfill % Fill the rest of the page with whitespace

  \end{titlepage}

  \begin{enumerate}
    \item Consider the function:
    \begin{equation}
      f(t)=\begin{cases}
      0~, ~~~~0< t < 1 \\
      1, ~~~~1< t< 2 
      \end{cases}
    \end{equation}
    Consider it to be periodic with period equaling the range of $t$ given above (i.e., $0<t<2$). Find the (real) Fourier series for $f(t)$.

      \textcolor{hwColor}{
        $f(x)=a_0+\sum\limits_{n=1}^{\infty}\left[a_n cos(\dfrac{n\pi}{L}x)+b_n sin(\dfrac{n\pi}{L}x)\right]$
      }

      \textcolor{hwColor}{
        $a_0=\dfrac{1}{2L}\bigints_{-L}^{L}f(x)dx$ \\
        $a_n=\dfrac{1}{L}\bigints_{-L}^{L}f(x) cos(\dfrac{n\pi}{L}x)dx$ \\
        $b_n=\dfrac{1}{L}\bigints_{-L}^{L}f(x) sin(\dfrac{n\pi}{L}x)dx$ \\
      }

      \textcolor{hwColor}{ 
        \rule{15cm}{0.4pt} 
      }

      \textcolor{hwColor}{ 
        P=2L $\Longrightarrow L=1$ \\
        \\
        $a_0=\dfrac{1}{2(1)}\bigints_{-1}^{1}f(x)dx=\dfrac{1}{2}\left[\bigints_{-1}^{0}f(x)dx+\bigints_{0}^{1}f(x)dx\right]$ \\
        $=\dfrac{1}{2}\left[\bigints_{-1}^{0}1.dx+\bigints_{0}^{1}0dx\right]=\dfrac{1}{2}\left[0-(-1)+0\right]$ \\
        $\Longrightarrow a_0=\dfrac{1}{2}$
      }

      \bigbreak

      \textcolor{hwColor}{ 
        $a_n=\bigints_{-1}^{1}f(x) cos(n\pi x)dx=\bigints_{-1}^{0}1.cos(n\pi x)dx+\bigints_{0}^{1}0.cos(n\pi x)dx=(\dfrac{sin(n\pi x)}{n\pi})\Big|_{-1}^{0}$ \\
        $=0-\dfrac{sin(-n\pi)}{n\pi}=\dfrac{sin(n\pi)}{n\pi}=\dfrac{0}{n\pi}$ \\
        \\
        $\Longrightarrow a_n=0$
      }

      \bigbreak

      \textcolor{hwColor}{ 
        $b_n=\bigints_{-1}^{1}f(x) sin(n\pi x)dx=\bigints_{-1}^{0}1.sin(n\pi x)dx+\bigints_{0}^{1}0.sin(n\pi x)dx=(\dfrac{-cos(n\pi x)}{n\pi})\Big|_{-1}^{0}$ \\
        $-\dfrac{cos(0)}{n\pi}+\dfrac{cos(-n\pi)}{n\pi}=-\dfrac{cos(0)}{n\pi}+\dfrac{cos(n\pi)}{n\pi}=-\dfrac{cos(0)}{n\pi}+\dfrac{(-1)^n}{n\pi}$\\
        \\
        $\Longrightarrow b_n=\begin{cases}
          0,~~~ 2n \\
          -\dfrac{2}{n\pi}, ~~~ 2n-1 
        \end{cases}$
      }

      \textcolor{hwColor}{ 
        $
          \Longrightarrow f(x)=\dfrac{1}{2}+\sum\limits_{n=1}^{\infty}b_n sin(n\pi x)
        $
      }

    \item Same as the previous exercise, for 
    \begin{equation}
      f(t)=\begin{cases}
      t~, ~~~~0< t < 1 \\
      t-2, ~~~~1< t< 2 
      \end{cases}
    \end{equation}

      \textcolor{hwColor}{
        $f(t)=\dfrac{a_0}{2}+\sum\limits_{r=1}^{\infty}\left[a_r cos(\dfrac{2\pi r}{L}t)+b_r sin(\dfrac{2\pi r}{L}t)\right]$
      }

      \textcolor{hwColor}{
        $a_0=\dfrac{2}{L}\bigints_{x_0}^{x_0+L}f(t)dt$ \\
        $a_r=\dfrac{2}{L}\bigints_{x_0}^{x_0+L}f(t) cos(\dfrac{2\pi r}{L}t)dt$ \\
        $b_r=\dfrac{2}{L}\bigints_{x_0}^{x_0+L}f(t) sin(\dfrac{2\pi r}{L}t)dt$ \\
      }

      \textcolor{hwColor}{ 
        \rule{15cm}{0.4pt} 
      }

      \textcolor{hwColor}{ 
        L=2 \\
        \\
        $a_0=\dfrac{2}{2}\bigints_{0}^{2}f(t)dt=\bigints_{0}^{1}tdt+\bigints_{1}^{2}(t-2)dt=\dfrac{1}{2}+(-2-(-\dfrac{3}{2}))$ \\
        \\ 
        $\Longrightarrow a_0=0$
      }

      \bigbreak

      \textcolor{hwColor}{
        $a_r=\dfrac{2}{2}\bigints_{0}^{2}f(t) cos(\pi rt)dt=\bigints_{0}^{1}t cos(\pi rt)dt+\bigints_{1}^{2}(t-2) cos(\pi rt)dt$ \\
        $=\left[\dfrac{t sin(\pi rt)}{\pi r}-\bigints \dfrac{sin(\pi rt)}{\pi r}dt=\dfrac{t sin(\pi rt)}{\pi r}+\dfrac{cos(\pi rt)}{(\pi r)^2}\right]\Big|_{0}^{1}$ \\
        $+\left[(t-2)\dfrac{sin(\pi rt)}{\pi r}-\bigints \dfrac{sin(\pi rt)}{\pi r}dt=(t-2)\dfrac{sin(\pi rt)}{\pi r}+\dfrac{cos(\pi rt)}{(\pi r)^2}\right]\Big|_{1}^{2}$ \\
      }

      \bigbreak

      \textcolor{hwColor}{
        $=\left[\dfrac{sin(\pi r)}{\pi r}+\dfrac{cos(\pi r)}{(\pi r)^2}-(0+\dfrac{1}{(\pi r)^2})=\dfrac{(-1)^r}{(\pi r)^2}-\dfrac{1}{(\pi r)^2}\right]$ \\
        $+\left[0+\dfrac{cos(2\pi r)}{(\pi r)^2}-(-\dfrac{sin(\pi r)}{\pi r}+\dfrac{cos(\pi r)}{(\pi r)^2})=\dfrac{1}{(\pi r)^2}+\dfrac{(-1)^r}{(\pi r)^2}\right]$
      }

      \bigbreak

      \textcolor{hwColor}{
        $=\dfrac{(-1)^r-1}{(\pi r)^2}+\dfrac{(-1)^r+1}{(\pi r)^2}$ \\
        \\
        $\Longrightarrow a_r=\dfrac{2(-1)^r}{(\pi r)^2}$
      }

      \bigbreak

      \textcolor{hwColor}{
        $b_r=\dfrac{2}{2}\bigints_{0}^{2}f(t) sin(\pi rt)dt=\bigints_{0}^{1}t sin(\pi rt)dt+\bigints_{1}^{2}(t-2) sin(\pi rt)dt$ \\
        $=\left[-\dfrac{tcos(\pi rt)}{\pi r}+\bigints\dfrac{cos(\pi rt)}{\pi r}dt=-\dfrac{t cos(\pi rt)}{\pi r}+\dfrac{sin(\pi rt)}{(\pi r)^2}\right]\Big|_{0}^{1}$ \\
        $+\left[-\dfrac{(t-2)cos(\pi rt)}{\pi r}+\bigints\dfrac{cos(\pi rt)}{\pi r}dt=-\dfrac{(t-2)cos(\pi rt)}{\pi r}+\dfrac{sin(\pi rt)}{(\pi r)^2}\right]\Big|_{1}^{2}$
      }

      \bigbreak

      \textcolor{hwColor}{
        $=\left[-(\dfrac{cos(\pi r)}{\pi r}+\dfrac{sin(\pi r)}{(\pi r)^2})-(-\dfrac{t}{\pi r}+0)=-\dfrac{(-1)^r}{\pi r}+\dfrac{t}{\pi r}\right]$ \\
        $+\left[(0+\dfrac{sin(2\pi r)}{(\pi r)^2})-(\dfrac{cos(\pi r)}{\pi r}+\dfrac{sin(\pi r)}{(\pi r)^2})=-\dfrac{(-1)^r}{\pi r}\right]$
      }

      \bigbreak

      \textcolor{hwColor}{
        $=\dfrac{t-(-1)^r}{\pi r}+\dfrac{-(-1)^r}{\pi r}=\dfrac{t-(-1)^r-(-1)^r}{\pi r}$ \\
        \\
        $\Longrightarrow b_r=\dfrac{t-2(-1)^r}{\pi r}$
      }


    \item Find the \emph{complex} Fourier series of the following periodic function (attention: recall that, outside the range given below, the function is repeated, see examples shown in class)
      \begin{equation}
      f(t)=\sin t~, ~~~~0< t < \pi \\
      \end{equation}

      \textcolor{hwColor}{
        $f(t)=\sum\limits_{r=-\infty}^{\infty} c_r~exp(\dfrac{2\pi irt}{L})$ \\
        \\
        $c_r=\dfrac{1}{L} \bigints_{x_0}^{x_0+L}f(t) ~ exp(-\dfrac{2\pi irt}{L}) dt$
      }

      \textcolor{hwColor}{ 
        \rule{15cm}{0.4pt} 
      }
      
      \textcolor{hwColor}{
        $L=\pi$ \\
        $c_r=\dfrac{1}{\pi} \bigints_{0}^{\pi}sin(t) ~ e^{(-\dfrac{2\pi irt}{\pi})} dt$
      }

      \bigbreak

      \textcolor{hwColor}{
        $\bigints sin(t) ~ e^{(-\dfrac{2\pi irt}{\pi})} dt=\bigints sin(t) ~ e^{(-2irt)} dt$ \\
        \\
        $=-e^{(-2irt)} cos(t)-2ir \bigints cost(t) e^{(-2irt)} dt=-e^{(-2irt)} cos(t)-2ir\left[e^{(-2irt)} sin(t)+2ir \bigints e^{(-2irt)} sin(t) dt\right]$ \\
        \\
        If $W=\bigints sin(t) ~ e^{(-2irt)} dt$, then we have \\
        \\
        $W=-e^{(-2irt)} cos(t)-2ir\left[e^{(-2irt)} sin(t)+2ir W\right]$\\
        \\
        $W+(2ir)^2W=-e^{(-2irt)} cos(t)-2ir ~ e^{(-2irt)} sin(t)$\\
        \\
        $\Longrightarrow \bigints sin(t) ~ e^{(-2irt)} dt=\dfrac{-e^{(-2irt)} cos(t)-2ire^{(-2irt)} sin(t)}{1+(2ir)^2}$
      }

      \bigbreak

      \textcolor{hwColor}{
        $c_r=\dfrac{1}{\pi} \bigints_{0}^{\pi}sin(t) ~ e^{(-2irt)} dt=\dfrac{1}{\pi} \left[\dfrac{-e^{(-2irt)} cos(t)-2ire^{(-2irt)} sin(t)}{1+(2ir)^2}\right]\Big|_{0}^{\pi}$ \\
        \\
        $=\dfrac{1}{\pi} \left[(\dfrac{-e^{(-2ir \pi)} cos(\pi)-2ire^{(-2ir \pi)} sin(\pi)}{1+(2ir)^2})-(\dfrac{-e^0 cos(0)-2ire^0 sin(0)}{1+(2ir)^2})\right]$ \\
        \\
        $=\dfrac{1}{\pi} \left[\dfrac{e^{i(-2r\pi)}+1}{1+(2ir)^2}\right]=\dfrac{1}{\pi}\left[\dfrac{cos(-2r\pi)+isin(-2r\pi)+1}{1+(2ir)^2}\right]=\dfrac{1}{\pi}\left[\dfrac{2}{1+(2ir)^2}\right]$ \\
        \\
        $\Longrightarrow c_r=\dfrac{2}{\pi \left[1+(2ir)^2\right]}$
      }


      \textcolor{hwColor}{
        Hence, the \emph{complex} Fourier series of the function is $f(t)=\sum\limits_{r=-\infty}^{\infty} \dfrac{2}{\pi \left[1+(2ir)^2\right]}~e^{2irt}$ \\
      }

      

    \item Find the \emph{complex} Fourier series of the following periodic function: 
    \begin{equation}
      f(t)=\begin{cases}
      0~, ~~~~0< t < \pi \\
      \sin t, ~~~~\pi< t< 2 \pi
      \end{cases}
    \end{equation}


  \end{enumerate}
\end{document}
