\documentclass[fleqn]{article}
\oddsidemargin 0.0in
\textwidth 6.0in
\thispagestyle{empty}
\usepackage{import}
\usepackage{amsmath}
\usepackage{graphicx}
\usepackage[english]{babel}
\usepackage[utf8x]{inputenc}
\usepackage{float}
\usepackage[colorinlistoftodos]{todonotes}

\definecolor{hwColor}{HTML}{AD53BA}

\begin{document}

  \begin{titlepage}

    \newcommand{\HRule}{\rule{\linewidth}{0.5mm}}

    \center
    


    \textsc{\LARGE Arizona State University}\\[1.5cm]

    \textsc{\LARGE Mathematical Methods For Physics I }\\[1.5cm]


    \begin{figure}
      \includegraphics[width=\linewidth]{asu.png}
    \end{figure}


    \HRule \\[0.4cm]
    { \huge \bfseries Homework 12}\\[0.4cm] 
    \HRule \\[1.5cm]
    
    \textbf{Behnam Amiri}

    \bigbreak

    \textbf{Prof: Cecilia Lunardini}

    \bigbreak


    \textbf{{\large \today}\\[2cm]}

    \vfill

  \end{titlepage}

  \begin{enumerate}
    \item Find the general solution of the equation: $\ddot y-3\dot y+2y=1+2 e^{3t}$ (here the dots indicate derivatives: $\dot y=dy/dt$, $\ddot y=d^2y/dt^2$).

      \textcolor{hwColor}{
        $
          \dfrac{d^2 y}{dt^2}-3\dfrac{dy}{dt}+2y=1+2e^{3t} \\
          \\
          y(t)=y_c(t)+y_p(t) \\
        $
      }

      \textcolor{hwColor}{
        The auxiliary equation: \\
        \\
        $
          \dfrac{d^2 (e^{\lambda t})}{dt^2}-3\dfrac{d(e^{\lambda t})}{dt}+2(e^{\lambda t})=0 \\
          \\
          \lambda^2 e^{\lambda t}-3\lambda e^{\lambda t}+2e^{\lambda t}=0 \rightarrow e^{\lambda t} \left[\lambda^2-3\lambda+2\right]=0 \\
          \\
          \lambda^2-3\lambda+2=0 \Longrightarrow \begin{cases}
            \lambda_1=1 \\
            \lambda_2=2
          \end{cases} \rightarrow 
          y_c(t)=c_1e^{\lambda_1 t}+c_2e^{\lambda_2 t}=c_1e^t+c_2e^{2t} \\
          \\
          y_c(t)=c_1e^t+c_2e^{2t}
        $
      }

      \bigbreak

      \textcolor{hwColor}{
        Let $y_p(x)=Ae^{3t}+B ~~~~ \dfrac{dy_p}{dt}=3Ae^{3t}~, ~~ \dfrac{d^2 y_p}{dt^2}=9Ae^{3t}$ \\
        $
          \dfrac{d^2 y}{dt^2}-3\dfrac{dy}{dt}+2y=9Ae^{3t}-3(3Ae^{3t})+2(Ae^{3t}+B)=1+2e^{3t} \\
          \\
          9Ae^{3t}-9Ae^{3t}+2Ae^{3t}+2B=1+2e^{3t} \\
          \\
          2Ae^{3t}+2B=1+2e^{3t} \rightarrow \begin{cases}
            2Ae^{3t}=2e^{3t}   \\
            2B=1  
          \end{cases} \Longrightarrow \begin{cases}
            A=1 \\
            B=\dfrac{1}{2}
          \end{cases} \\
          \\
          y_p(x)=e^{3t}+\dfrac{1}{2} \\
          \\
          y(t)=y_c(t)+y_p(t)=c_1e^t+c_2e^{2t}+e^{3t}+\dfrac{1}{2} \\
          \\
          \\
          \Longrightarrow y(t)=c_1e^t+c_2e^{2t}+e^{3t}+\dfrac{1}{2}
        $
      }
      
    \item Solve the following inhomogeneous differential equations. Give the general solution and then apply the conditions:

      \begin{enumerate}
        \item $\ddot y-4 \dot y+3y=t; ~~~~~~ y(0)=1, ~ \dot y(0)=0.$

          \textcolor{hwColor}{
            $
              \dfrac{d^2 y}{dt^2}-4\dfrac{dy}{dt}+3y=t \\
              \\
              y(t)=y_c(t)+y_p(t) \\
            $
          }

          \textcolor{hwColor}{
            The auxiliary equation: \\
            \\
            $
              \dfrac{d^2 (e^{\lambda t})}{dt^2}-4\dfrac{d(e^{\lambda t})}{dt}+3(e^{\lambda t})=0 \\
              \\
              \lambda^2 e^{\lambda t}-4\lambda e^{\lambda t}+3e^{\lambda t}=0 \rightarrow e^{\lambda t} \left[\lambda^2-4\lambda+3\right]=0 \\
              \\
              \lambda^2-4\lambda+3=0 \Longrightarrow \begin{cases}
                \lambda_1=1 \\
                \lambda_2=3
              \end{cases} \rightarrow 
              y_c(t)=c_1e^{\lambda_1 t}+c_2e^{\lambda_2 t}=c_1e^t+c_2e^{3t} \\
              \\
              y_c(t)=c_1e^t+c_2e^{3t}
            $
          }

          \bigbreak

          \textcolor{hwColor}{
            Let $y_p(x)=At+B ~~~~ \dfrac{dy_p}{dt}=A~, ~~ \dfrac{d^2 y_p}{dt^2}=0$ \\
            $
              \dfrac{d^2 y}{dt^2}-4\dfrac{dy}{dt}+3y=0-4(A)+3(At+B)=t \rightarrow \begin{cases}
                3A=1   \\
                3B-4A=0  
              \end{cases} \Longrightarrow \begin{cases}
                A=\dfrac{1}{3} \\
                B=\dfrac{4}{9}
              \end{cases} \\
              \\
              y_p(x)=\dfrac{1}{3}t+\dfrac{4}{9} \\
              \\
              y(t)=y_c(t)+y_p(t)=c_1e^t+c_2e^{3t}+\dfrac{1}{3}t+\dfrac{4}{9} \\
              \\
              \\
              \Longrightarrow y(t)=c_1e^t+c_2e^{3t}+\dfrac{1}{3}t+\dfrac{4}{9}
            $
          }

          \bigbreak

          \textcolor{hwColor}{
            $
              \dfrac{d(y(t))}{dt}=c_1e^t+3c_2e^{3t}+\dfrac{1}{3}, ~~~~ y(0)=1, ~ \dot y(0)=0 \\ \\
              \\
              y(0)=c_1e^0+c_2e^{0}+(\dfrac{1}{3})0+\dfrac{4}{9}=1 \rightarrow c_1+c_2+\dfrac{4}{9}=1 \Longrightarrow c_1+c_2=\dfrac{5}{9} \\
              \\
              \dot y(0)=c_1e^0+3c_2e^0+\dfrac{1}{3}=0 \rightarrow c_1+3c_2=-\dfrac{1}{3} \\
              \\
              \begin{cases}
                c_1+c_2=\dfrac{5}{9} \\
                c_1+3c_2=-\dfrac{1}{3} 
              \end{cases} \Longrightarrow \begin{cases}
                c_1=1 \\
                c_2=-\dfrac{4}{9}
              \end{cases} \\
              \\
              \\
              \Longrightarrow y(t)=e^t-\dfrac{4}{9}e^{3t}+\dfrac{1}{3}t+\dfrac{4}{9}
            $
          }

        \item $\ddot y-4y=2cos(t) ~~~~~~ y(0)=0, ~ \dot y(0)=0.$

          \textcolor{hwColor}{
            $
              \dfrac{d^2 y}{dt^2}-4y=2cos(t) \\
              \\
              y(t)=y_c(t)+y_p(t) \\
            $
          }

          \textcolor{hwColor}{
            The auxiliary equation: \\
            \\
            $
              \dfrac{d^2 (e^{\lambda t})}{dt^2}-4e^{\lambda t}=0 \\
              \\
              \lambda^2 e^{\lambda t}-4e^{\lambda t}=0 \rightarrow e^{\lambda t} \left[\lambda^2-4\right]=0 \\
              \\
              \lambda^2-4=0 \Longrightarrow \begin{cases}
                \lambda_1=-2 \\
                \lambda_2=+2
              \end{cases} \rightarrow 
              y_c(t)=c_1e^{\lambda_1 t}+c_2e^{\lambda_2 t}=c_1e^{-2t}+c_2e^{2t} \\
              \\
              y_c(t)=c_1e^{-2t}+c_2e^{2t}
            $
          }

          \bigbreak

          \textcolor{hwColor}{
            Let $y_p(x)=Acos(t)+Bsin(t) ~~~~ \dfrac{dy_p}{dt}=-Asin(t)+Bsin(t), ~~ \dfrac{d^2 y_p}{dt^2}=-\left[Acos(t)+Bsin(t)\right]$ \\
            $
              \dfrac{d^2 y}{dt^2}-4(Acos(t)+Bsin(t))=2cos(t) \\
              \\
              -Acos(t)-Bsin(t)-4Acos(t)-4Bsin(t)=2cos(t) \\
              \\
              -5Acos(t)-5bsin(t)=2cos(t)
              \rightarrow \begin{cases}
                -5A=2   \\
                -5B=0  
              \end{cases} \Longrightarrow \begin{cases}
                A=-\dfrac{2}{5} \\
                B=0
              \end{cases} \\
              \\
              y_p(x)=-\dfrac{2}{5}cos(t) \\
              \\
              y(t)=y_c(t)+y_p(t)=c_1e^{-2t}+c_2e^{2t}-\dfrac{2}{5}cos(t) \\
              \\
              \\
              \Longrightarrow y(t)=c_1e^{-2t}+c_2e^{2t}-\dfrac{2}{5}cos(t)
            $
          }

          \bigbreak

          \textcolor{hwColor}{
            $
              \dfrac{d(y(t))}{dt}=-2c_1e^{-2t}+2c_2e^{2t}+\dfrac{2}{5}sin(t), ~~~~ y(0)=0, ~ \dot y(0)=0 \\ \\
              \\
              y(0)=c_1e^{0}+c_2e^{0}-\dfrac{2}{5}cos(0)=0 \rightarrow c_1+c_2=\dfrac{2}{5} \\
              \\
              \dot y(0)=-2c_1e^{0}+2c_2e^{0}+\dfrac{2}{5}sin(0)=0 \rightarrow -2c_1+2c_2=0 \\
              \\
              \begin{cases}
                c_1+c_2=\dfrac{2}{5} \\
                -2c_1+2c_2=0 
              \end{cases} \Longrightarrow \begin{cases}
                c_1=\dfrac{1}{5} \\
                \\
                c_2=\dfrac{1}{5}
              \end{cases} \\
              \\
              \\
              \Longrightarrow y(t)=\dfrac{1}{5}e^{-2t}+\dfrac{1}{5}e^{2t}-\dfrac{2}{5}cos(t)
            $
          }

        \item $\ddot y+4\dot y+3y=4e^{-t} ~~~~~~ y(0)=0, ~ \dot y(0)=2.$

          \textcolor{hwColor}{
            $
              \dfrac{d^2 y}{dt^2}+4\dfrac{dy}{dt}+3y=4e^{-t} \\
              \\
              y(t)=y_c(t)+y_p(t) \\
            $
          }

          \textcolor{hwColor}{
            The auxiliary equation: \\
            \\
            $
              \dfrac{d^2 (e^{\lambda t})}{dt^2}+4\dfrac{d(e^{\lambda t})}{dt}+3(e^{\lambda t})=0 \\
              \\
              \lambda^2 e^{\lambda t}+4\lambda e^{\lambda t}+3(e^{\lambda t})=0 \rightarrow e^{\lambda t} \left[\lambda^2+4\lambda+3\right]=0 \\
              \\
              \lambda^2+4\lambda+3 \Longrightarrow \begin{cases}
                \lambda_1=-1 \\
                \lambda_2=-3
              \end{cases} \rightarrow 
              y_c(t)=c_1e^{\lambda_1 t}+c_2e^{\lambda_2 t}=c_1e^{-t}+c_2e^{-3t} \\
              \\
              y_c(t)=c_1e^{-t}+c_2e^{-3t}
            $
          }

          \bigbreak

          \textcolor{hwColor}{
            Let $y_p(x)=tAe^{-t} ~~~~ \dfrac{dy_p}{dt}=Ae^{-t}-tAe^{-t} \\ 
            \dfrac{d^2 y_p}{dt^2}=-Ae^{-t}-(Ae^{-t}-tAe^{-t})=-2Ae^{-t}+tAe^{-t}$ \\
            \\
            $
              -2Ae^{-t}+tAe^{-t}+4(Ae^{-t}-tAe^{-t})+3(tAe^{-t})=4e^{-t} \\
              \\
              -2Ae^{-t}+tAe^{-t}+4Ae^{-t}-4tAe^{-t})+3tAe^{-t}=4e^{-t} \\
              \\
              2A+tA-4tA+3tA=4 \\
              \rightarrow \begin{cases}
                A=2   \\
              \end{cases}
              \\
              y_p(x)=2te^{-t} \\
              \\
              y(t)=y_c(t)+y_p(t)=c_1e^{-t}+c_2e^{-3t}+2te^{-t} \\
              \\
              \Longrightarrow y(t)=c_1e^{-t}+c_2e^{-3t}+2te^{-t}
            $
          }

          \bigbreak

          \textcolor{hwColor}{
            $
              \dfrac{d(y(t))}{dt}=-c_1e^{-t}-3c_2e^{-3t}+2e^{-t}-2te^{-t} ~~~~ y(0)=0, ~ \dot y(0)=2 \\ \\
              \\
              y(0)=c_1e^{0}+c_2e^{0}+2(0)e^{0}=c_1+c_2=0 \\
              \\
              \dot y(0)=-c_1e^{0}-3c_2e^{0}+2e^{0}-2(0)e^{0}=-c_1-3c_2+2=2 \\
              \\
              \begin{cases}
                c_1+c_2=0 \\
                -c_1-3c_2=0 
              \end{cases} \Longrightarrow \begin{cases}
                c_1=0 \\
                c_2=0
              \end{cases} \\
              \\
              \\
              \Longrightarrow y(t)=2te^{-t}
            $
          }
              
        \item $\ddot y+2 \dot y+6y=3tsin(2t) ~~~~~~ y(0)=1, ~ \dot y(0)=2.$
      \end{enumerate}

    \item Refer to the reading on the driven oscillator posted on Canvas (see Module 22 file recommended\_reading\_driven\_oscillator.pdf), and do the exercises 26, 27 and 28 there. 

    \item Refer to the reading on the driven oscillator posted on Canvas (see Module 22 file recommended\_reading\_driven\_oscillator.pdf), and do the exercises 29 and 30 there. 
          
  \end{enumerate}

\end{document}
